backends/lean/Base/Primitives/Core.lean
@@ -22,7 +22,7 @@ structure Index (Self Idx : Type) where
 /- Trait declaration: [core::ops::index::IndexMut] -/
 structure IndexMut (Self Idx : Type) where
   indexInst : Index Self Idx
-  index_mut : Self → Idx → Result (indexInst.Output × (indexInst.Output → Result Self))
+  index_mut : Self → Idx → Result (indexInst.Output × (indexInst.Output → Self))
 
 end index -- core.ops.index
 
@@ -34,7 +34,7 @@ structure Deref (Self : Type) where
 
 structure DerefMut (Self : Type) where
   derefInst : Deref Self
-  deref_mut : Self → Result (derefInst.Target × (Self → Result Self))
+  deref_mut : Self → Result (derefInst.Target × (Self → Self))
 
 end deref -- core.ops.deref
 
